Integrate Sambin modalised-context uniqueness into Tiling.v
Folds ModalSambin.v into the Sambin-uniqueness section after sambin_uniform_uniqueness_boxed: modalised_in_p, the box-substitution congruence box_subst_iff_lift, outer_subst_iff, sambin_uniqueness_modalised and its box-atomic/Loeb-form corollaries. Removes ModalSambin.v.

Tiling.v
@@ -19085,6 +19085,259 @@ Proof.
   apply (sambin_uniform_uniqueness_base p phi); assumption.
 Qed.
 
+(** ** Sambin uniqueness for arbitrary modalised contexts.
+
+    [sambin_uniqueness_modalised]: every C : Form -> Form arising by
+    substitution in some [phi] with [modalized p phi] admits at most one
+    fixed point up to provable equivalence.  Structural induction on phi,
+    Loeb at level 0 once for the outer descent; the Box case goes through
+    the congruence [box_subst_iff_lift], proved by structural induction
+    on chi without a modalisation hypothesis. *)
+
+Definition modalised_in_p (C : Form -> Form) : Prop :=
+  exists (p : nat) (phi : Form),
+    modalized p phi /\ forall psi, C psi = Subst p psi phi.
+
+Lemma Subst_Var_explicit : forall p k psi,
+  Subst p psi (Var k) = (if Nat.eqb k p then psi else Var k).
+Proof. intros. unfold Subst. simpl. reflexivity. Qed.
+
+Lemma Subst_Impl_eq : forall p psi X Y,
+  Subst p psi (Impl X Y) = Impl (Subst p psi X) (Subst p psi Y).
+Proof. intros. unfold Subst. simpl. reflexivity. Qed.
+
+Lemma Subst_Box_eq : forall p psi i chi,
+  Subst p psi (Box i chi) = Box i (Subst p psi chi).
+Proof. intros. unfold Subst. simpl. reflexivity. Qed.
+
+Lemma Subst_Bot_eq : forall p psi, Subst p psi Bot = Bot.
+Proof. intros. reflexivity. Qed.
+
+Lemma prov_box_chain_internal : forall A B C j,
+  |- Impl A (Box j B) ->
+  |- Impl A (Box j (Impl B C)) ->
+  |- Impl A (Box j C).
+Proof.
+  intros A B C j HB HBC.
+  pose proof (Ax_BoxK j B C) as HK.
+  pose proof (prov_compose _ _ _ HBC HK) as HBC2.
+  pose proof (Ax_S A (Box j B) (Box j C)) as Hs.
+  pose proof (MP _ _ Hs HBC2) as HSBC.
+  exact (MP _ _ HSBC HB).
+Qed.
+
+Lemma prov_impl_chain_S : forall A B C,
+  |- Impl A (Impl B C) -> |- Impl A B -> |- Impl A C.
+Proof.
+  intros A B C HABC HAB.
+  pose proof (Ax_S A B C) as Hs.
+  pose proof (MP _ _ Hs HABC) as Hs2.
+  exact (MP _ _ Hs2 HAB).
+Qed.
+
+Lemma prov_box_0_to_box_j_box_0 : forall j phi,
+  |- Impl (Box 0 phi) (Box j (Box 0 phi)).
+Proof.
+  intros j phi.
+  pose proof (Ax_Box4 0 phi) as H4.
+  pose proof (prov_box_mon_le 0 j (Box 0 phi) (Nat.le_0_l j)) as Hmon.
+  exact (prov_compose _ _ _ H4 Hmon).
+Qed.
+
+Lemma iff_trans_atomic :
+  |- Impl (Iff (Var 0) (Var 1))
+       (Impl (Iff (Var 1) (Var 2)) (Iff (Var 0) (Var 2))).
+Proof.
+  apply trivial_in_provable. apply prop_completeness.
+  - cbn. unfold Iff, And, Neg. cbn. tauto.
+  - intro val. cbn. unfold Iff, And, Neg. cbn.
+    destruct (val 0), (val 1), (val 2); reflexivity.
+Qed.
+
+Lemma iff_trans_internal : forall a b c,
+  |- Impl (Iff a b) (Impl (Iff b c) (Iff a c)).
+Proof.
+  intros a b c.
+  pose proof (subst_provable
+    (fun n => match n with | 0 => a | 1 => b | _ => c end)
+    _ iff_trans_atomic) as H.
+  cbn in H. exact H.
+Qed.
+
+Lemma impl_iff_compat_atomic :
+  |- Impl (Iff (Var 0) (Var 1))
+       (Impl (Iff (Var 2) (Var 3))
+             (Iff (Impl (Var 0) (Var 2)) (Impl (Var 1) (Var 3)))).
+Proof.
+  apply trivial_in_provable. apply prop_completeness.
+  - cbn. unfold Iff, And, Neg. cbn. tauto.
+  - intro val. cbn. unfold Iff, And, Neg. cbn.
+    destruct (val 0), (val 1), (val 2), (val 3); reflexivity.
+Qed.
+
+Lemma impl_iff_compat_internal : forall X1 X2 Y1 Y2,
+  |- Impl (Iff X1 X2)
+       (Impl (Iff Y1 Y2)
+             (Iff (Impl X1 Y1) (Impl X2 Y2))).
+Proof.
+  intros X1 X2 Y1 Y2.
+  pose proof (subst_provable
+    (fun n => match n with
+              | 0 => X1 | 1 => X2 | 2 => Y1 | _ => Y2 end)
+    _ impl_iff_compat_atomic) as H.
+  cbn in H. exact H.
+Qed.
+
+Lemma iff_chain_under : forall A a b c,
+  |- Impl A (Iff a b) ->
+  |- Impl A (Iff b c) ->
+  |- Impl A (Iff a c).
+Proof.
+  intros A a b c Hab Hbc.
+  pose proof (iff_trans_internal a b c) as Htrans.
+  pose proof (prov_compose _ _ _ Hab Htrans) as Hstep1.
+  exact (prov_impl_chain_S A (Iff b c) (Iff a c) Hstep1 Hbc).
+Qed.
+
+(** Box-substitution congruence: for any [chi] and level [j],
+    [Box 0 (Iff psi1 psi2)] entails
+    [Box j (Iff (chi[psi1]) (chi[psi2]))].  Structural induction on
+    [chi]. *)
+
+Lemma box_subst_iff_lift : forall (p : nat) (psi1 psi2 : Form) (chi : Form) (j : nat),
+  |- Impl (Box 0 (Iff psi1 psi2))
+          (Box j (Iff (Subst p psi1 chi) (Subst p psi2 chi))).
+Proof.
+  intros p psi1 psi2 chi.
+  induction chi as [k | | X IHX Y IHY | i chi' IHchi]; intro j.
+  - rewrite !Subst_Var_explicit.
+    destruct (Nat.eqb k p) eqn:Ekp.
+    + exact (prov_box_mon_le 0 j (Iff psi1 psi2) (Nat.le_0_l j)).
+    + pose proof (prov_iff_refl (Var k)) as Hrefl.
+      pose proof (Nec j _ Hrefl) as Hnec.
+      exact (prov_weaken _ (Box 0 (Iff psi1 psi2)) Hnec).
+  - rewrite !Subst_Bot_eq.
+    pose proof (prov_iff_refl Bot) as Hrefl.
+    pose proof (Nec j _ Hrefl) as Hnec.
+    exact (prov_weaken _ (Box 0 (Iff psi1 psi2)) Hnec).
+  - rewrite !Subst_Impl_eq.
+    pose proof (IHX j) as IH_X.
+    pose proof (IHY j) as IH_Y.
+    pose proof (impl_iff_compat_internal
+                  (Subst p psi1 X) (Subst p psi2 X)
+                  (Subst p psi1 Y) (Subst p psi2 Y)) as Hcompat.
+    pose proof (Nec j _ Hcompat) as HcompatN.
+    pose proof (Ax_BoxK j (Iff (Subst p psi1 X) (Subst p psi2 X))
+                  (Impl (Iff (Subst p psi1 Y) (Subst p psi2 Y))
+                        (Iff (Impl (Subst p psi1 X) (Subst p psi1 Y))
+                             (Impl (Subst p psi2 X) (Subst p psi2 Y))))) as HK1.
+    pose proof (MP _ _ HK1 HcompatN) as Hstep1.
+    pose proof (prov_compose _ _ _ IH_X Hstep1) as Hstep2.
+    exact (prov_box_chain_internal _ _ _ _ IH_Y Hstep2).
+  - rewrite !Subst_Box_eq.
+    pose proof (IHchi i) as IH.
+    pose proof (Nec j _ IH) as IHN.
+    pose proof (Ax_BoxK j (Box 0 (Iff psi1 psi2))
+                  (Box i (Iff (Subst p psi1 chi') (Subst p psi2 chi')))) as HK1.
+    pose proof (MP _ _ HK1 IHN) as Hstep1.
+    pose proof (prov_box_0_to_box_j_box_0 j (Iff psi1 psi2)) as HB0Bj.
+    pose proof (prov_compose _ _ _ HB0Bj Hstep1) as Hstep2.
+    pose proof (box_iff_distrib i (Subst p psi1 chi') (Subst p psi2 chi')) as Hdist.
+    pose proof (Nec j _ Hdist) as HdistN.
+    pose proof (Ax_BoxK j (Box i (Iff (Subst p psi1 chi') (Subst p psi2 chi')))
+                  (Iff (Box i (Subst p psi1 chi')) (Box i (Subst p psi2 chi')))) as HK2.
+    pose proof (MP _ _ HK2 HdistN) as Hstep3.
+    exact (prov_compose _ _ _ Hstep2 Hstep3).
+Qed.
+
+(** With the modalisation hypothesis on phi, the substituted iff is
+    provable directly under [Box 0 (Iff psi1 psi2)]; the Box case appeals
+    to [box_subst_iff_lift]. *)
+
+Lemma outer_subst_iff : forall (p : nat) (psi1 psi2 : Form) (phi : Form),
+  modalized p phi ->
+  |- Impl (Box 0 (Iff psi1 psi2))
+          (Iff (Subst p psi1 phi) (Subst p psi2 phi)).
+Proof.
+  intros p psi1 psi2 phi.
+  induction phi as [k | | X IHX Y IHY | i chi IHchi]; intro Hmod; cbn in Hmod.
+  - rewrite !Subst_Var_explicit.
+    destruct (Nat.eqb k p) eqn:Ekp.
+    + apply Nat.eqb_eq in Ekp. subst k. exfalso. apply Hmod. reflexivity.
+    + pose proof (prov_iff_refl (Var k)) as Hrefl.
+      exact (prov_weaken _ (Box 0 (Iff psi1 psi2)) Hrefl).
+  - rewrite !Subst_Bot_eq.
+    pose proof (prov_iff_refl Bot) as Hrefl.
+    exact (prov_weaken _ (Box 0 (Iff psi1 psi2)) Hrefl).
+  - destruct Hmod as [HmX HmY].
+    pose proof (IHX HmX) as IH_X.
+    pose proof (IHY HmY) as IH_Y.
+    rewrite !Subst_Impl_eq.
+    pose proof (impl_iff_compat_internal
+                  (Subst p psi1 X) (Subst p psi2 X)
+                  (Subst p psi1 Y) (Subst p psi2 Y)) as Hcompat.
+    pose proof (prov_compose _ _ _ IH_X Hcompat) as Hstep1.
+    exact (prov_impl_chain_S _ _ _ Hstep1 IH_Y).
+  - rewrite !Subst_Box_eq.
+    pose proof (box_subst_iff_lift p psi1 psi2 chi i) as Hmaster.
+    pose proof (box_iff_distrib i (Subst p psi1 chi) (Subst p psi2 chi)) as Hdist.
+    exact (prov_compose _ _ _ Hmaster Hdist).
+Qed.
+
+Theorem sambin_uniqueness_modalised : forall (C : Form -> Form),
+  modalised_in_p C ->
+  forall psi1 psi2,
+    |- Iff psi1 (C psi1) ->
+    |- Iff psi2 (C psi2) ->
+    |- Iff psi1 psi2.
+Proof.
+  intros C HC psi1 psi2 Hfp1 Hfp2.
+  destruct HC as [p [phi [Hmod Heq]]].
+  rewrite Heq in Hfp1, Hfp2.
+  apply (loeb_metatheorem 0 (Iff psi1 psi2)).
+  pose proof (outer_subst_iff p psi1 psi2 phi Hmod) as Houter.
+  pose proof (prov_weaken _ (Box 0 (Iff psi1 psi2)) Hfp1) as Hfp1_w.
+  pose proof (prov_iff_sym _ _ Hfp2) as Hfp2_sym.
+  pose proof (prov_weaken _ (Box 0 (Iff psi1 psi2)) Hfp2_sym) as Hfp2_w.
+  pose proof (iff_chain_under _ psi1 (Subst p psi1 phi) (Subst p psi2 phi)
+                Hfp1_w Houter) as Hstep1.
+  exact (iff_chain_under _ psi1 (Subst p psi2 phi) psi2 Hstep1 Hfp2_w).
+Qed.
+
+(** The headline subsumes the single-class uniqueness theorems for
+    Box-atomic and Loeb-form contexts. *)
+
+Corollary sambin_uniqueness_modalised_box_atomic : forall n psi1 psi2,
+  |- Iff psi1 (Box n psi1) ->
+  |- Iff psi2 (Box n psi2) ->
+  |- Iff psi1 psi2.
+Proof.
+  intros n psi1 psi2 H1 H2.
+  apply (sambin_uniqueness_modalised (fun X => Box n X)).
+  - exists 0, (Box n (Var 0)). split.
+    + cbn. exact I.
+    + intro psi. unfold Subst. simpl. reflexivity.
+  - exact H1.
+  - exact H2.
+Qed.
+
+Corollary sambin_uniqueness_modalised_loeb_form : forall n X psi1 psi2,
+  ~ In 0 (free_vars X) ->
+  |- Iff psi1 (Box n (Impl psi1 X)) ->
+  |- Iff psi2 (Box n (Impl psi2 X)) ->
+  |- Iff psi1 psi2.
+Proof.
+  intros n X psi1 psi2 HnoX H1 H2.
+  apply (sambin_uniqueness_modalised (fun Y => Box n (Impl Y X))).
+  - exists 0, (Box n (Impl (Var 0) X)). split.
+    + cbn. exact I.
+    + intro psi. unfold Subst. simpl.
+      pose proof (Subst_no_occurrence 0 psi X HnoX) as HX.
+      unfold Subst in HX. rewrite HX. reflexivity.
+  - exact H1.
+  - exact H2.
+Qed.
+
 Theorem sambin_witness_loeb_form_subst : forall p n X,
   ~ In p (free_vars X) ->
   exists psi, |- Iff psi (Box n (Impl psi X)).
